making progress on functional version

examples/MutableBtree.dfy
@@ -6,7 +6,7 @@ include "../lib/Maps.dfy"
 
 abstract module MutableBtree {
   import opened NativeTypes
-  import opened Sequences
+  import opened Seq = Sequences
   import opened Maps
   import Arrays
   import Keys : Total_Order
@@ -32,655 +32,953 @@ abstract module MutableBtree {
   {
     //assert false;
   }
-    
-  trait Node {
-    ghost var subtreeObjects: set<object>
-    ghost var allKeys: set<Key>
-      
-    predicate WF()
-      reads this, subtreeObjects
-      ensures WF() ==> this in subtreeObjects
-      decreases subtreeObjects, 0
 
-    // function QueryDef(needle: Key) : QueryResult
-    //   requires WF()
-    //   reads this, subtreeObjects
-    //   decreases subtreeObjects
-      
-    function Interpretation() : map<Key, Value>
-      requires WF()
-      // ensures forall key :: QueryDef(key).Found? ==> MapsTo(Interpretation(), key, QueryDef(key).value)
-      // ensures forall key :: QueryDef(key).NotFound? ==> key !in Interpretation()
-      reads this, subtreeObjects
-      decreases subtreeObjects
-
-    method Query(needle: Key) returns (result: QueryResult)
-      requires WF()
-      //ensures result == QueryDef(needle)
-      ensures needle in Interpretation() ==> result == Found(Interpretation()[needle])
-      ensures needle !in Interpretation() ==> result == NotFound
-      decreases subtreeObjects
-
-    predicate method Full()
-      requires WF()
-      reads this, subtreeObjects
-      
-    method Insert(key: Key, value: Value)
-      requires WF()
-      requires !Full()
-      ensures WF()
-      ensures Interpretation() == old(Interpretation())[key := value]
-      ensures allKeys == old(allKeys) + {key}
-      ensures fresh(subtreeObjects-old(subtreeObjects))
-      modifies this, subtreeObjects
-      decreases allKeys
-      
-    static function MergeMaps(left: map<Key, Value>, pivot: Key, right: map<Key, Value>) : map<Key, Value> {
-      map key |
-        && key in left.Keys + right.Keys
-        && (|| (Keys.lt(key, pivot) && key in left)
-           || (Keys.lte(pivot, key) && key in right))
-         ::
-         if Keys.lt(key, pivot) && key in left then left[key]
-         else right[key]
-    }
-    
-    predicate SplitEnsures(oldint: map<Key, Value>, pivot: Key, rightnode: Node)
-      reads this, subtreeObjects
-      reads rightnode, rightnode.subtreeObjects
-    {
-      && WF()
-      && !Full()
-      && rightnode.WF()
-      && !rightnode.Full()
-      && MergeMaps(Interpretation(), pivot, rightnode.Interpretation()) == oldint
-      && allKeys != {}
-      && rightnode.allKeys != {}
-      && (forall key :: key in allKeys ==> Keys.lt(key, pivot))
-      && (forall key :: key in rightnode.allKeys ==> Keys.lte(pivot, key))
-    }
-      
-    method Split() returns (ghost wit: Key, pivot: Key, rightnode: Node)
-      requires WF()
-      requires Full()
-      ensures SplitEnsures(old(Interpretation()), pivot, rightnode)
-      ensures allKeys <= old(allKeys)
-      ensures rightnode.allKeys <= old(allKeys)
-      ensures pivot in old(allKeys)
-      ensures wit in old(allKeys)
-      ensures Keys.lt(wit, pivot)
-      ensures subtreeObjects <= old(subtreeObjects)
-      ensures subtreeObjects !! rightnode.subtreeObjects
-      ensures fresh(rightnode.subtreeObjects - old(subtreeObjects))
-      modifies this
-  }
-
-  datatype NodeBox = NodeBox(node: Node?)
-
-  class Leaf extends Node {
-    var nkeys : uint64
-    var keys: array<Key>
-    var values: array<Value>
-
-    predicate WF()
-      reads this, subtreeObjects
-      ensures WF() ==> this in subtreeObjects
-      decreases subtreeObjects, 0
-    {
-      && subtreeObjects == {this, keys, values}
-      && keys != values
-      && keys.Length == MaxKeysPerLeaf() as int
-      && values.Length == MaxKeysPerLeaf() as int
-      && 0 <= nkeys <= keys.Length as uint64
-      && Keys.IsStrictlySorted(keys[..nkeys])
-      && allKeys == set key | key in multiset(keys[..nkeys])
-    }
-
-    // function QueryDef(needle: Key) : (result: QueryResult)
-    //   requires WF()
-    //   reads subtreeObjects
-    // {
-    //   var pos: int := Keys.LargestLte(keys[..nkeys], needle);
-    //   if 0 <= pos && keys[pos] == needle then Found(values[pos])
-    //   else NotFound
-    // }
-    
-    function Interpretation() : map<Key, Value>
-      requires WF()
-      // ensures forall key :: QueryDef(key).Found? ==> MapsTo(Interpretation(), key, QueryDef(key).value)
-      // ensures forall key :: QueryDef(key).NotFound? ==> key !in Interpretation()
-      reads this, subtreeObjects
-      decreases subtreeObjects
-    {
-      Keys.PosEqLargestLteForAllElts(keys[..nkeys]);
-      map k | (k in keys[..nkeys]) :: values[Keys.LargestLte(keys[..nkeys], k)]
-    }
-
-
-    method Query(needle: Key) returns (result: QueryResult)
-      requires WF()
-      ensures needle in Interpretation() ==> result == Found(Interpretation()[needle])
-      ensures needle !in Interpretation() ==> result == NotFound
-      //ensures result == QueryDef(needle)
-      decreases subtreeObjects
-    {
-      //Keys.reveal_IsStrictlySorted();
-      var posplus1: uint64 := Keys.ArrayLargestLtePlus1(keys, 0, nkeys, needle);
-      if 1 <= posplus1 && keys[posplus1-1] == needle {
-        result := Found(values[posplus1-1]);
-      } else {
-        result := NotFound;
-      }
-    }
-
-    predicate method Full()
-      requires WF()
-      reads this, subtreeObjects
-    {
-      nkeys >= MaxKeysPerLeaf()
-    }
-    
-    method Insert(key: Key, value: Value)
-      requires WF()
-      requires !Full()
-      ensures WF()
-      ensures Interpretation() == old(Interpretation())[key := value]
-      ensures allKeys == old(allKeys) + {key}
-      ensures fresh(subtreeObjects-old(subtreeObjects))
-      modifies this, subtreeObjects
-      decreases allKeys
-    {
-      var posplus1 := Keys.ArrayLargestLtePlus1(keys, 0, nkeys, key);
-
-      if 1 <= posplus1 && keys[posplus1-1] == key {
-        values[posplus1-1] := value;
-      } else {
-        ghost var oldkeys := keys[..nkeys];
-        Arrays.Insert(keys, nkeys, key, posplus1);
-        Arrays.Insert(values, nkeys, value, posplus1);
-        nkeys := nkeys + 1;
-        allKeys := allKeys + {key};
-
-        InsertMultiset(oldkeys, key, posplus1 as int); // OBSERVE
-        Keys.strictlySortedInsert(oldkeys, key, posplus1 as int - 1); // OBSERVE
-        Keys.PosEqLargestLte(keys[..nkeys], key, posplus1 as int);
-        forall key' |  key' != key && key' in old(Interpretation())
-          ensures key' in Interpretation() && Interpretation()[key'] == old(Interpretation())[key']
-        {
-          var i: int := Keys.LargestLte(old(keys[..nkeys]), key');
-          //assert 0 <= i;
-          if i < posplus1 as int {
-            //assert keys[i] == key';
-            Keys.PosEqLargestLte(keys[..nkeys], key', i);
-          } else {
-            //assert keys[i+1] == key';
-            Keys.PosEqLargestLte(keys[..nkeys], key', i+1);
-          }
-        }
-        forall key' | key' != key && key' in Interpretation()
-          ensures key' in old(Interpretation()) && old(Interpretation())[key'] == Interpretation()[key']
-        {
-          var i: int := Keys.LargestLte(keys[..nkeys], key');
-          if i < posplus1 as int {
-            Keys.PosEqLargestLte(old(keys[..nkeys]), key', i);
-          } else {
-            Keys.PosEqLargestLte(old(keys[..nkeys]), key', i-1);
-          }
-        }
-      }
-    }
-
-    method Split() returns (ghost wit: Key, pivot: Key, rightnode: Node)
-      requires WF()
-      requires Full()
-      ensures SplitEnsures(old(Interpretation()), pivot, rightnode)
-      ensures allKeys <= old(allKeys)
-      ensures rightnode.allKeys <= old(allKeys)
-      ensures pivot in old(allKeys)
-      ensures wit in old(allKeys)
-      ensures Keys.lt(wit, pivot)
-      ensures subtreeObjects <= old(subtreeObjects)
-      ensures subtreeObjects !! rightnode.subtreeObjects
-      ensures fresh(rightnode.subtreeObjects - old(subtreeObjects))
-      modifies this
-    {
-      var right := new Leaf();
-      var boundary := nkeys/2;
-      Arrays.Memcpy(right.keys, 0, keys[boundary..nkeys]); // FIXME: remove conversion to seq
-      Arrays.Memcpy(right.values, 0, values[boundary..nkeys]); // FIXME: remove conversion to seq
-      right.nkeys := nkeys - boundary;
-      nkeys := boundary;
-      allKeys := set key | key in multiset(keys[..nkeys]);
-      right.allKeys := set key | key in multiset(right.keys[..right.nkeys]);
-      assert keys[0] in allKeys;
-      assert right.keys[0] in right.allKeys;
-      wit := keys[0];
-      pivot := right.keys[0];
-      rightnode := right;
-
-      assert keys[..nkeys] == old(keys[..nkeys])[..nkeys];
-      Keys.StrictlySortedSubsequence(old(keys[..nkeys]), 0, nkeys as int);
-      assert WF();
-      assert right.keys[..right.nkeys] == old(keys[..nkeys])[boundary..old(nkeys)];
-      Keys.StrictlySortedSubsequence(old(keys[..nkeys]), boundary as int, old(nkeys) as int);
-      assert Keys.IsStrictlySorted(right.keys[..right.nkeys]);
-      assert right.WF();
-      Keys.IsStrictlySortedImpliesLt(old(keys[..nkeys]), 0, boundary as int);
-      forall i | 0 <= i < nkeys
-        ensures Keys.lt(keys[i], pivot)
-      {
-        Keys.IsStrictlySortedImpliesLt(old(keys[..nkeys]), i as int, boundary as int);
-      }
-      ghost var mergedint := MergeMaps(Interpretation(), pivot, rightnode.Interpretation());
-      forall key | key in old(Interpretation())
-        ensures key in mergedint && mergedint[key] == old(Interpretation())[key]
-      {
-        if Keys.lt(key, pivot) {
-          assert Keys.LargestLte(old(keys[..nkeys]), key) < boundary as int;
-        } else {
-        }
-      }
-    }
-      
-    constructor()
-      ensures WF()
-      ensures Interpretation() == map[]
-      ensures !Full()
-      ensures fresh(keys)
-      ensures fresh(values)
-    {
-      nkeys := 0;
-      keys := new Key[MaxKeysPerLeaf()](_ => DefaultKey());
-      values := new Value[MaxKeysPerLeaf()](_ => DefaultValue());
-      allKeys := {};
-      subtreeObjects := {this, keys, values};
-    }
-  }
-
-  class Index extends Node {
-    var nchildren: uint64
-    var pivots: array<Key>
-    var children: array<NodeBox>
-
-    predicate WF()
-      reads this, subtreeObjects
-      ensures WF() ==> this in subtreeObjects
-      decreases subtreeObjects, 0
-    {
-      && {this, pivots, children} <= subtreeObjects
-      && pivots.Length == (MaxChildren() as int) - 1
-      && children.Length == MaxChildren() as int
-      && 1 <= nchildren <= MaxChildren()
-      && Keys.IsStrictlySorted(pivots[..nchildren-1])
-      && (forall i :: 0 <= i < nchildren ==> children[i].node != null)
-      && (forall i :: 0 <= i < nchildren ==> children[i].node in subtreeObjects)
-      && (forall i {:trigger children[i].node.subtreeObjects} :: 0 <= i < nchildren as int ==> children[i].node.subtreeObjects < subtreeObjects)
-      && (forall i {:trigger children[i].node.subtreeObjects} :: 0 <= i < nchildren as int ==> {this, pivots, children} !! children[i].node.subtreeObjects)
-      && (forall i :: 0 <= i < nchildren ==> children[i].node.WF())
-      && (forall i, j {:trigger children[i].node.subtreeObjects, children[j].node.subtreeObjects} :: 0 <= i < j < nchildren as int ==> children[i].node.subtreeObjects !! children[j].node.subtreeObjects)
-      && (forall i :: 0 <= i < nchildren ==> children[i].node.allKeys != {})
-      && (forall i :: 0 <= i < nchildren ==> children[i].node.allKeys < allKeys)
-      && (forall i, key :: 0 <= i < nchildren-1 && key in children[i].node.allKeys ==> Keys.lt(key, pivots[i]))
-      && (forall i, key :: 0 < i < nchildren   && key in children[i].node.allKeys ==> Keys.lte(pivots[i-1], key))
-
-    }
-
-    // lemma AllKeysStrictlyDecreasing()
-    //   requires WF()
-    //   ensures forall i :: 0 <= i < nchildren ==> children[i].node.allKeys < allKeys
-    // {
-    //   forall i | 0 <= i < nchildren
-    //     ensures children[i].node.allKeys < allKeys
-    //   {
-    //     var i' := if i < nchildren-1 then i+1 else 0;
-    //     assert i' != i;
-    //     assert children[i].node.allKeys !! children[i'].node.allKeys;
-    //     assert children[i].node.allKeys <= 
-    //     assert children[i].node.allKeys <= allKeys;
-    //   }
-    // }
-    
-    // function QueryDef(needle: Key) : QueryResult
-    //   requires WF()
-    //   reads this, subtreeObjects
-    //   decreases subtreeObjects
-    // {
-    //   var pos := Keys.LargestLte(pivots[..nchildren-1], needle);
-    //   children[pos + 1].node.QueryDef(needle)
-    // }
-    
-    function Interpretation() : (result: map<Key, Value>)
-      requires WF()
-      // ensures forall key :: QueryDef(key).Found? ==> MapsTo(result, key, QueryDef(key).value)
-      // ensures forall key :: QueryDef(key).NotFound? ==> key !in Interpretation()
-      reads this, subtreeObjects
-      decreases subtreeObjects
-    {
-      // This is just to prove finiteness.  Thanks to James Wilcox for the trick:
-      // https://stackoverflow.com/a/47585360
-      var allkeys := set key, i | 0 <= i < nchildren && key in children[i].node.Interpretation() :: key;
-      var result := map key |
-        && key in allkeys
-        && key in children[Keys.LargestLte(pivots[..nchildren-1], key) + 1].node.Interpretation()
-        :: children[Keys.LargestLte(pivots[..nchildren-1], key) + 1].node.Interpretation()[key];
-
-      // assert forall key :: QueryDef(key).Found? ==> key in children[Keys.LargestLte(pivots[..nchildren-1], key)+1].node.Interpretation();
-        
-      result
-    }
-
-    method Query(needle: Key) returns (result: QueryResult)
-      requires WF()
-      ensures needle in Interpretation() ==> result == Found(Interpretation()[needle])
-      ensures needle !in Interpretation() ==> result == NotFound
-      // ensures result == QueryDef(needle)
-      decreases subtreeObjects
-    {
-      var posplus1 := Keys.ArrayLargestLtePlus1(pivots, 0, nchildren-1, needle);
-      result := children[posplus1].node.Query(needle);
-    }
-
-    predicate method Full()
-      requires WF()
-      reads this, subtreeObjects
-    {
-      nchildren == MaxChildren()
-    }
-
-    method SplitChild(key: Key, childidx: uint64) returns (newchildidx: uint64)
-      requires WF()
-      requires !Full()
-      requires childidx as int == 1 + Keys.LargestLte(pivots[..nchildren-1], key)
-      requires children[childidx].node.Full()
-      ensures WF()
-      ensures Interpretation() == old(Interpretation())
-      ensures newchildidx as int == 1 + Keys.LargestLte(pivots[..nchildren-1], key)
-      ensures !children[newchildidx].node.Full()
-      ensures allKeys == old(allKeys)
-      ensures fresh(subtreeObjects-old(subtreeObjects))
-      modifies this, pivots, children, children[childidx].node
-    {
-      ghost var oldchildren := children[..nchildren];
-      
-      var wit, pivot, right := children[childidx].node.Split();
-      Arrays.Insert(pivots, nchildren - 1, pivot, childidx);
-      Arrays.Insert(children, nchildren, NodeBox(right), childidx + 1);
-      nchildren := nchildren + 1;
-      subtreeObjects := subtreeObjects + right.subtreeObjects;
-      if Keys.lte(pivot, key) {
-        newchildidx := childidx + 1;
-      } else {
-        newchildidx := childidx;
-      }
-
-      Keys.LargestLteIsUnique(old(pivots[..nchildren-1]), pivot, childidx as int - 1);
-      Keys.strictlySortedInsert(old(pivots[..nchildren-1]), pivot, childidx as int - 1);
-
-      assert forall i :: 0 <= i < childidx as int ==> children[i] == oldchildren[i];
-      assert children[childidx as int + 1].node == right;
-      assert forall i :: childidx as int + 1 < i < nchildren as int  ==> children[i] == oldchildren[i-1];
-      forall i: int, j: int {:trigger children[i].node.subtreeObjects, children[j].node.subtreeObjects}
-      | 0 <= i < j < nchildren as int
-        ensures children[i].node.subtreeObjects !! children[j].node.subtreeObjects
-      {
-        if                                   j  < childidx as int {
-        } else if                            j == childidx as int {
-        } else if i  < childidx as int     && j == childidx as int + 1 {
-        } else if i == childidx as int     && j == childidx as int + 1 {
-        } else if i  < childidx as int     && j  > childidx as int + 1 {
-        } else if i == childidx as int     && j  > childidx as int + 1 {
-        } else if i == childidx as int + 1 && j  > childidx as int + 1 {
-        } else {
-        }
-      }
-      // forall i: int, key | 0 <= i < (nchildren as int)-1 && key in children[i].node.allKeys
-      //   ensures Keys.lt(key, pivots[i])
-      // {
-      //   if childidx as int + 1 < i {
-      //     assert children[i] == old(children[i-1]);
-      //   }
-      // }
-      // forall i: int, key | 0 < i < nchildren as int && key in children[i].node.allKeys
-      //   ensures Keys.lt(pivots[i-1], key)
-      // {
-      //   if i < childidx as int {
-      //     assert Keys.lt(pivots[i-1], key);
-      //   } else if i == childidx as int {
-      //     assert Keys.lt(pivots[i-1], key);
-      //   } else if i == childidx as int + 1 {
-      //     assert Keys.lt(pivots[i-1], key);
-      //   } else {
-      //     assert Keys.lt(pivots[i-1], key);
-      //   }
-      // }
-      assert WF();
-        
-      forall key | key in old(Interpretation())
-        ensures key in Interpretation() && Interpretation()[key] == old(Interpretation()[key])
-      {
-        var llte: int := Keys.LargestLte(old(pivots[..nchildren-1]), key);
-        assert key in old(children[llte+1].node.Interpretation());
-        assert old(children[llte+1].node.Interpretation()[key]) == old(Interpretation()[key]);
-        if llte < childidx as int {
-          assert key in Interpretation() && Interpretation()[key] == old(Interpretation()[key]);
-        } else if llte == childidx as int {
-          if Keys.lt(key, pivot) {
-            assert key in Interpretation() && Interpretation()[key] == old(Interpretation()[key]);
-          } else {
-            assert key in Interpretation() && Interpretation()[key] == old(Interpretation()[key]);
-          }
-        } else {
-          assert key in Interpretation() && Interpretation()[key] == old(Interpretation()[key]);
-        }
-      }
-      forall key | key in Interpretation()
-        ensures key in old(Interpretation()) && Interpretation()[key] == old(Interpretation()[key])
-      {
-        var llte: int := Keys.LargestLte(pivots[..nchildren-1], key);
-        if llte < childidx as int {
-        } else if llte == childidx as int {
-        } else if llte == childidx as int + 1 {
-        } else {
-        }
-      }
-    }
-    
-    method Insert(key: Key, value: Value)
-      requires WF()
-      requires !Full()
-      ensures WF()
-      ensures Interpretation() == old(Interpretation())[key := value]
-      ensures allKeys == old(allKeys) + {key}
-      ensures fresh(subtreeObjects - old(subtreeObjects))
-      modifies this, subtreeObjects
-      decreases allKeys
-    {
-      var posplus1 := Keys.ArrayLargestLtePlus1(pivots, 0, nchildren - 1, key);
-      var childidx := (posplus1) as uint64;
-      if children[posplus1].node.Full() {
-        childidx := SplitChild(key, childidx);
-      }
-      //AllKeysStrictlyDecreasing();
-      children[childidx].node.Insert(key, value);
-      subtreeObjects := subtreeObjects + children[childidx].node.subtreeObjects;
-      allKeys := allKeys + {key};
-      forall key' | key' in old(Interpretation()) && key' != key
-        ensures key' in Interpretation() && Interpretation()[key'] == old(Interpretation()[key'])
-      {
-        var i :| 0 <= i < old(nchildren) && key' in old(children[i].node.Interpretation());
-      }
-      
-    }
-
-    function UnionSubtreeObjects() : set<object>
-      requires nchildren as int <= children.Length
-      requires forall i :: 0 <= i < nchildren ==> children[i].node != null
-      reads this, children, set i | 0 <= i < nchildren :: children[i].node
-    {
-      set o, i | 0 <= i < nchildren && o in children[i].node.subtreeObjects :: o
-    }
-    
-    method Split() returns (ghost wit: Key, pivot: Key, rightnode: Node)
-      requires WF()
-      requires Full()
-      ensures SplitEnsures(old(Interpretation()), pivot, rightnode)
-      ensures allKeys <= old(allKeys)
-      ensures rightnode.allKeys <= old(allKeys)
-      ensures pivot in old(allKeys)
-      ensures wit in old(allKeys)
-      ensures Keys.lt(wit, pivot)
-      ensures subtreeObjects <= old(subtreeObjects)
-      ensures subtreeObjects !! rightnode.subtreeObjects
-      ensures fresh(rightnode.subtreeObjects - old(subtreeObjects))
-      modifies this
-    {
-      var right := new Index();
-      var boundary := nchildren/2;
-      Arrays.Memcpy(right.pivots, 0, pivots[boundary..nchildren-1]); // FIXME: remove conversion to seq
-      Arrays.Memcpy(right.children, 0, children[boundary..nchildren]); // FIXME: remove conversion to seq
-      right.nchildren := nchildren - boundary;
-      nchildren := boundary;
-      subtreeObjects := {this, pivots, children} + UnionSubtreeObjects();
-      right.subtreeObjects := right.subtreeObjects + right.UnionSubtreeObjects();
-
-      pivot := pivots[boundary-1];
-
-      right.allKeys := set k | k in allKeys && Keys.lte(pivot, k);
-      allKeys := set k | k in allKeys && Keys.lt(k, pivot);
-      
-      wit := right.pivots[0];
-      rightnode := right;
-      AssumeFalse();
-      
-      // Keys.reveal_IsStrictlySorted();
-      // assert WF();
-      // assert rightnode.WF();
-      // assert MergeMaps(Interpretation(), pivot, rightnode.Interpretation()) == old(Interpretation());
-    }
-
-    constructor()
-      ensures nchildren == 0
-      ensures pivots.Length == (MaxChildren() as int)-1
-      ensures children.Length == (MaxChildren() as int)
-      ensures forall i :: 0 <= i < children.Length ==> children[i].node == null
-      ensures subtreeObjects == {this, pivots, children}
-      ensures allKeys == {}
-      ensures fresh(pivots)
-      ensures fresh(children)
-    {
-      pivots := new Key[MaxChildren()-1](_ => DefaultKey());
-      children := new NodeBox[MaxChildren()](_ => NodeBox(null));
-      nchildren := 0;
-      subtreeObjects := {this, pivots, children};
-      allKeys := {};
-    }
-  }
-
-  class MutableBtree {
-    var root: Node
-
-    function Interpretation() : map<Key, Value>
-      requires root.WF()
-      reads this, root, root.subtreeObjects
-    {
-      root.Interpretation()
-    }
-
-    method Query(needle: Key) returns (result: QueryResult)
-      requires root.WF()
-      ensures result == NotFound ==> needle !in Interpretation()
-      ensures result.Found? ==> needle in Interpretation() && Interpretation()[needle] == result.value
-    {
-      result := root.Query(needle);
-    }
-
-    method Insert(key: Key, value: Value)
-      requires root.WF()
-      ensures root.WF()
-      ensures Interpretation() == old(Interpretation())[key := value]
-      modifies this, root, root.subtreeObjects
-    {
-      if root.Full() {
-        var newroot := new Index();
-        newroot.children[0] := NodeBox(root);
-        newroot.nchildren := 1;
-        newroot.subtreeObjects := newroot.subtreeObjects + root.subtreeObjects;
-        newroot.allKeys := root.allKeys;
-        root := newroot;
-      }
-      AssumeFalse();
-      root.Insert(key, value);
-    }
-    
-    constructor()
-      ensures root.WF()
-      ensures Interpretation() == map[]
-    {
-      root := new Leaf();
-    }
-  }
-}
-
-module TestMutableBtree refines MutableBtree {
-  import Keys = Uint64_Order
-  type Value = uint64
-
-  function method MaxKeysPerLeaf() : uint64 { 64 }
-  function method MaxChildren() : uint64 { 64 }
-
-  function method DefaultValue() : Value { 0 }
-  function method DefaultKey() : Key { 0 }
-}
-
-module MainModule {
-  import opened NativeTypes
-  import TestMutableBtree
-    
-  method Main()
+  datatype ImmutableNode =
+    | ImmutableLeaf(keys: seq<Key>, values: seq<Value>)
+    | ImmutableIndex(pivots: seq<Key>, children: seq<ImmutableNode>)
+  
+  function AllKeysNode(node: ImmutableNode) : set<Key>
   {
-    // var n: uint64 := 1_000_000;
-    // var p: uint64 := 300_007;
-    var n: uint64 := 10_000_000;
-    var p: uint64 := 3_000_017;
-    // var n: uint64 := 100_000_000;
-    // var p: uint64 := 1_073_741_827;
-    var t := new TestMutableBtree.MutableBtree();
-    var i: uint64 := 0;
-    while i < n
-      invariant 0 <= i <= n
-      invariant t.root.WF()
-      modifies t, t.root, t.root.subtreeObjects
+    match node {
+      case ImmutableLeaf(keys, values) => set k | k in keys
+      case ImmutableIndex(pivots, children) => set i, k | 0 <= i < |children| && k in AllKeysNode(children[i]) :: k
+    }    
+  }
+  
+  predicate WFLeaf(leaf: ImmutableNode)
+    requires leaf.ImmutableLeaf?
+  {
+    && |leaf.keys| == |leaf.values|
+    && Keys.IsStrictlySorted(leaf.keys)
+  }
+
+  predicate WFIndex(index: ImmutableNode)
+    requires index.ImmutableIndex?
+    decreases index, 0
+  {
+    && |index.pivots| == |index.children| - 1
+    && Keys.IsStrictlySorted(index.pivots)
+    && (forall i :: 0 <= i < |index.children| ==> WFNode(index.children[i]))
+    && (forall i :: 0 <= i < |index.children| ==> AllKeysNode(index.children[i]) != {})
+    && (forall i, key :: 0 <= i < |index.children|-1 && key in AllKeysNode(index.children[i]) ==> Keys.lt(key, index.pivots[i]))
+    && (forall i, key :: 0 < i < |index.children|   && key in AllKeysNode(index.children[i]) ==> Keys.lte(index.pivots[i-1], key))
+  }
+
+  predicate WFNode(node: ImmutableNode)
+    decreases node, 1
+  {
+    match node {
+      case ImmutableLeaf(_, _) =>  WFLeaf(node)
+      case ImmutableIndex(_, _) => WFIndex(node)
+    }
+  }
+
+  function InterpretLeaf(leaf: ImmutableNode) : map<Key, Value>
+    requires leaf.ImmutableLeaf?
+    requires WFLeaf(leaf)
+  {
+    Keys.PosEqLargestLteForAllElts(leaf.keys);
+    map k | (k in leaf.keys) :: leaf.values[Keys.LargestLte(leaf.keys, k)]
+  }
+
+  function InterpretIndex(index: ImmutableNode) : map<Key, Value>
+    requires index.ImmutableIndex?
+    requires WFIndex(index)
+    decreases index, 0
+  {
+    map key |
+      && key in AllKeysNode(index)
+      && key in InterpretNode(index.children[Keys.LargestLte(index.pivots, key) + 1])
+      :: InterpretNode(index.children[Keys.LargestLte(index.pivots, key) + 1])[key]
+  }
+
+  function InterpretNode(node: ImmutableNode) : map<Key, Value>
+    requires WFNode(node)
+    decreases node, 1
+  {
+    match node {
+      case ImmutableLeaf(_, _) => InterpretLeaf(node)
+      case ImmutableIndex(_, _) => InterpretIndex(node)
+    }
+  }
+
+  function InsertLeaf(leaf: ImmutableNode, key: Key, value: Value) : (result: ImmutableNode)
+    requires leaf.ImmutableLeaf?
+    requires WFLeaf(leaf)
+    ensures result.ImmutableLeaf?
+    ensures WFLeaf(result)
+  {
+    var llte := Keys.LargestLte(leaf.keys, key);
+    if 0 <= llte && leaf.keys[llte] == key then
+      ImmutableLeaf(leaf.keys, leaf.values[llte := value])
+    else
+      Keys.strictlySortedInsert(leaf.keys, key, llte);
+      ImmutableLeaf(Seq.insert(leaf.keys, key, llte+1), Seq.insert(leaf.values, value, llte+1))
+  }
+
+  lemma InsertLeafIsCorrect(leaf: ImmutableNode, key: Key, value: Value, result: ImmutableNode)
+    requires leaf.ImmutableLeaf?
+    requires WFLeaf(leaf)
+    requires result == InsertLeaf(leaf, key, value)
+    ensures InterpretNode(result) == InterpretNode(leaf)[key := value]
+  {
+    var llte := Keys.LargestLte(leaf.keys, key);
+    if 0 <= llte && leaf.keys[llte] == key {
+      assert InterpretNode(result) == InterpretNode(leaf)[key := value];
+    } else {
+      Keys.reveal_IsStrictlySorted();
+      forall k | k in InterpretNode(result).Keys
+        ensures k in InterpretNode(leaf).Keys + {key}
+      {
+        var kpos := IndexOf(result.keys, k);
+        if llte + 1 < kpos {
+          assert k == leaf.keys[kpos-1];
+        }
+      }
+    }
+  }
+   
+  predicate SplitLeaf(oldleaf: ImmutableNode, leftleaf: ImmutableNode, rightleaf: ImmutableNode, pivot: Key)
+  {
+    && oldleaf.ImmutableLeaf?
+    && leftleaf.ImmutableLeaf?
+    && rightleaf.ImmutableLeaf?
+    && WFLeaf(oldleaf)
+    && WFLeaf(leftleaf)
+    && WFLeaf(rightleaf)
+    && 0 < |leftleaf.keys|
+    && 0 < |rightleaf.keys|
+    && oldleaf.keys == leftleaf.keys + rightleaf.keys
+    && oldleaf.values == leftleaf.values + rightleaf.values
+    && Keys.lt(Last(leftleaf.keys), pivot)
+    && Keys.lte(pivot, rightleaf.keys[0])
+  }
+
+  // lemma SplitLeafAllKeys(oldleaf: ImmutableNode, leftleaf: ImmutableNode, rightleaf: ImmutableNode, pivot: Key)
+  //   requires SplitLeaf(oldleaf, leftleaf, rightleaf, pivot)
+  //   ensures AllKeysNode(oldleaf) == AllKeysNode(leftleaf) + AllKeysNode(rightleaf)
+  //   ensures AllKeysNode(leftleaf) == set k | k in AllKeysNode(oldleaf) && Keys.lt(k, pivot)
+  //   ensures AllKeysNode(rightleaf) == set k | k in AllKeysNode(oldleaf) && Keys.lte(pivot, k)
+  // {
+  //   Keys.reveal_IsStrictlySorted();
+  // }
+
+  lemma SplitLeafInterpretation(oldleaf: ImmutableNode, leftleaf: ImmutableNode, rightleaf: ImmutableNode, pivot: Key)
+    requires SplitLeaf(oldleaf, leftleaf, rightleaf, pivot)
+    ensures InterpretLeaf(oldleaf) == MapDisjointUnion(InterpretLeaf(leftleaf), InterpretLeaf(rightleaf))
+  {
+    var oldint := InterpretLeaf(oldleaf);
+    var leftint := InterpretLeaf(leftleaf);
+    var rightint := InterpretLeaf(rightleaf);
+    var newint := MapDisjointUnion(leftint, rightint);
+
+    forall key | key in oldint
+      ensures newint[key] == oldint[key]
     {
-      t.Insert((i * p) % n , i);
-      i := i + 1;
+      var llte := Keys.LargestLte(oldleaf.keys, key);
+      if llte < |leftleaf.keys| {
+        Keys.PosEqLargestLte(leftleaf.keys, key, llte);
+      } else {
+        var rightllte := llte - |leftleaf.keys|;
+        Keys.PosEqLargestLte(rightleaf.keys, key, rightllte);
+      }
+    }
+  }
+  
+  predicate SplitIndex(oldindex: ImmutableNode, leftindex: ImmutableNode, rightindex: ImmutableNode, pivot: Key)
+  {
+    && oldindex.ImmutableIndex?
+    && leftindex.ImmutableIndex?
+    && rightindex.ImmutableIndex?
+    && WFIndex(oldindex)
+    && WFIndex(leftindex)
+    && WFIndex(rightindex)
+    && oldindex.pivots == leftindex.pivots + [pivot] + rightindex.pivots
+    && oldindex.children == leftindex.children + rightindex.children
+  }
+
+  // lemma SplitIndexAllKeys(oldindex: ImmutableNode, leftindex: ImmutableNode, rightindex: ImmutableNode, pivot: Key)
+  //   requires SplitIndex(oldindex, leftindex, rightindex, pivot)
+  //   ensures AllKeysNode(oldindex) == AllKeysNode(leftindex) + AllKeysNode(rightindex)
+  //   ensures AllKeysNode(leftindex) == set k | k in AllKeysNode(oldindex) && Keys.lt(k, pivot)
+  //   ensures AllKeysNode(rightindex) == set k | k in AllKeysNode(oldindex) && Keys.lte(pivot, k)
+  // {
+  //   assert AllKeysNode(oldindex) <= AllKeysNode(leftindex) + AllKeysNode(rightindex);
+  //   forall key | key in AllKeysNode(leftindex) + AllKeysNode(rightindex)
+  //     ensures key in AllKeysNode(oldindex)
+  //   {
+  //     if key in AllKeysNode(leftindex) {
+  //       var i :| 0 <= i < |leftindex.children| && key in AllKeysNode(leftindex.children[i]);
+  //       assert key in AllKeysNode(oldindex.children[i]);
+  //     } else {
+  //       var i :| 0 <= i < |rightindex.children| && key in AllKeysNode(rightindex.children[i]);
+  //       assert key in AllKeysNode(oldindex.children[|leftindex.children|+i]);
+  //     }
+  //   }
+  //   forall key | key in AllKeysNode(leftindex)
+  //     ensures Keys.lt(key, pivot)
+  //   {
+      
+  //   }
+  //   assert AllKeysNode(leftindex) <= set k | k in AllKeysNode(oldindex) && Keys.lt(k, pivot);
+  //   assert AllKeysNode(leftindex) >= set k | k in AllKeysNode(oldindex) && Keys.lt(k, pivot);
+  //   assert AllKeysNode(rightindex) <= set k | k in AllKeysNode(oldindex) && Keys.lte(pivot, k);
+  //   assert AllKeysNode(rightindex) >= set k | k in AllKeysNode(oldindex) && Keys.lte(pivot, k);
+  // }
+  
+  lemma SplitIndexInterpretation(oldindex: ImmutableNode, leftindex: ImmutableNode, rightindex: ImmutableNode, pivot: Key)
+    requires SplitIndex(oldindex, leftindex, rightindex, pivot)
+    ensures InterpretIndex(oldindex) == Keys.MapPivotedUnion(InterpretIndex(leftindex), pivot, InterpretIndex(rightindex))
+  {
+    var oldint := InterpretIndex(oldindex);
+    var leftint := InterpretIndex(leftindex);
+    var rightint := InterpretIndex(rightindex);
+    var newint := Keys.MapPivotedUnion(leftint, pivot, rightint);
+
+    Keys.reveal_IsStrictlySorted();
+    Keys.PosEqLargestLte(oldindex.pivots, pivot, |leftindex.pivots|);
+    
+    forall key | key in oldint
+      ensures MapsTo(newint, key, oldint[key])
+    {
+      if Keys.lt(key, pivot) {
+      } else {
+      }
     }
 
-    // i := 0;
-    // while i < n
-    //   invariant 0 <= i <= n
-    // {
-    //   var needle := (i * p) % n;
-    //   var qr := t.Query(needle);
-    //   if qr != TestMutableBtree.Found(i) {
-    //     print "Test failed";
-  //   } else {
-  //     //print "Query ", i, " for ", needle, "resulted in ", qr.value, "\n";
-  //   }
-  //   i := i + 1;
-  // }
-
-  // i := 0;
-  // while i < n
-  //   invariant 0 <= i <= n
-  // {
-  //   var qr := t.Query(n + ((i * p) % n));
-  //   if qr != TestMutableBtree.NotFound {
-  //     print "Test failed";
-  //   } else {
-  //     //print "Didn't return bullsh*t\n";
-  //   }
-  //   i := i + 1;
-  // }
-    print "PASSED\n";
+    forall key | key in newint
+      ensures MapsTo(oldint, key, newint[key])
+    {
+      if Keys.lt(key, pivot) {
+      } else {
+      }
+    }
+    
   }
+  
+  predicate SplitNode(oldnode: ImmutableNode, leftnode: ImmutableNode, rightnode: ImmutableNode, pivot: Key)
+  {
+    || SplitLeaf(oldnode, leftnode, rightnode, pivot)
+    || SplitIndex(oldnode, leftnode, rightnode, pivot)
+  }
+  
+  predicate SplitChildOfIndex(oldindex: ImmutableNode, newindex: ImmutableNode, childidx: int)
+  {
+    && oldindex.ImmutableIndex?
+    && newindex.ImmutableIndex?
+    && WFNode(oldindex)
+    && WFNode(newindex)
+    && 0 <= childidx < |oldindex.children|
+    && |newindex.children| == |oldindex.children| + 1 // FIXME: WTF?  Dafny can't get these from WFNode?
+    && |newindex.pivots| == |oldindex.pivots| + 1
+    && |oldindex.pivots| == |oldindex.children| - 1
+    && newindex.pivots == Seq.insert(oldindex.pivots, newindex.pivots[childidx], childidx)
+    && SplitNode(oldindex.children[childidx], newindex.children[childidx], newindex.children[childidx+1], newindex.pivots[childidx])
+    && newindex.children == oldindex.children[..childidx] + [newindex.children[childidx], newindex.children[childidx+1]] + oldindex.children[childidx+1..]
+  }
+
+  lemma SplitChildOfIndexPreservesInterpretation(oldindex: ImmutableNode, newindex: ImmutableNode, childidx: int)
+    requires SplitChildOfIndex(oldindex, newindex, childidx)
+    ensures InterpretNode(newindex) == InterpretNode(oldindex)
+  {
+    var newint := InterpretNode(newindex);
+    var oldint := InterpretNode(oldindex);
+    
+    assert WFIndex(oldindex); // WTF?  Dafny can't see these (from emacs flycheck mode)
+    assert WFIndex(newindex);
+
+    forall key | key in oldint
+      ensures key in newint && newint[key] == oldint[key]
+    {
+      assert key in InterpretIndex(oldindex);
+      var llte := Keys.LargestLte(oldindex.pivots, key);
+      var oldchild := oldindex.children[llte+1];
+      var oldchildint := InterpretNode(oldchild);
+      assert key in oldchildint;
+      assert oldint[key] == oldchildint[key];
+      if llte + 1 < childidx {
+        var newllte := llte;
+        assert newllte == Keys.LargestLte(newindex.pivots, key);
+        var newchildint := InterpretNode(newindex.children[newllte+1]);
+        assert newindex.children[newllte+1] == oldindex.children[llte+1];
+        assert newchildint == oldchildint;
+        assert key in newchildint;
+        assert key in AllKeysNode(newindex);
+        assert newint == InterpretIndex(newindex);
+        assert key in newint;
+        assert newint[key] == newchildint[key];
+      } else if llte + 1 == childidx {
+        assert key in AllKeysNode(oldchild);
+        var leftchild := newindex.children[childidx];
+        var rightchild := newindex.children[childidx+1];
+        assert key in AllKeysNode(leftchild) + AllKeysNode(rightchild);
+        if Keys.lt(key, newindex.pivots[childidx]) {
+          var newllte := llte;
+          assert newllte == Keys.LargestLte(newindex.pivots, key);
+          var newchild := leftchild;
+          var newchildint := InterpretNode(newchild);
+          assert key in AllKeysNode(newchild);
+          assert key in newchildint;
+          assert key in newint;
+          assert newint[key] == newchildint[key];
+        } else {
+          var newllte := llte + 1;
+          assert newllte == Keys.LargestLte(newindex.pivots, key);
+          assume false;
+        }
+      } else {
+        var newllte := llte + 1;
+        assert newllte == Keys.LargestLte(newindex.pivots, key);
+        var newchildint := InterpretNode(newindex.children[newllte+1]);
+        assert newindex.children[newllte+1] == oldindex.children[llte+1];
+        assert newchildint == oldchildint;
+        assert key in newchildint;
+        assert key in AllKeysNode(newindex);
+        assert newint == InterpretIndex(newindex);
+        assert key in newint;
+        assert newint[key] == newchildint[key];
+      }
+    }
+
+    forall key | key in newint
+      ensures key in oldint
+    {
+      assume false;
+    }
+  }
+    
+//   trait Node {
+//     ghost var subtreeObjects: set<object>
+//     ghost var allKeys: set<Key>
+
+//     function ToImmutableNode() : ImmutableNode
+//       reads this, subtreeObjects
+//       decreases subtreeObjects, 0
+      
+//     predicate WF()
+//       reads this, subtreeObjects
+//       ensures WF() ==> this in subtreeObjects
+//       decreases subtreeObjects, 0
+
+//     // function QueryDef(needle: Key) : QueryResult
+//     //   requires WF()
+//     //   reads this, subtreeObjects
+//     //   decreases subtreeObjects
+      
+//     function Interpretation() : map<Key, Value>
+//       requires WF()
+//       // ensures forall key :: QueryDef(key).Found? ==> MapsTo(Interpretation(), key, QueryDef(key).value)
+//       // ensures forall key :: QueryDef(key).NotFound? ==> key !in Interpretation()
+//       reads this, subtreeObjects
+//       decreases subtreeObjects
+
+//     method Query(needle: Key) returns (result: QueryResult)
+//       requires WF()
+//       //ensures result == QueryDef(needle)
+//       ensures needle in Interpretation() ==> result == Found(Interpretation()[needle])
+//       ensures needle !in Interpretation() ==> result == NotFound
+//       decreases subtreeObjects
+
+//     predicate method Full()
+//       requires WF()
+//       reads this, subtreeObjects
+      
+//     method Insert(key: Key, value: Value)
+//       requires WF()
+//       requires !Full()
+//       ensures WF()
+//       ensures Interpretation() == old(Interpretation())[key := value]
+//       ensures allKeys == old(allKeys) + {key}
+//       ensures fresh(subtreeObjects-old(subtreeObjects))
+//       modifies this, subtreeObjects
+//       decreases allKeys
+      
+//     predicate SplitEnsures(oldint: map<Key, Value>, pivot: Key, rightnode: Node)
+//       reads this, subtreeObjects
+//       reads rightnode, rightnode.subtreeObjects
+//     {
+//       && WF()
+//       && !Full()
+//       && rightnode.WF()
+//       && !rightnode.Full()
+//       && MergeMaps(Interpretation(), pivot, rightnode.Interpretation()) == oldint
+//       && allKeys != {}
+//       && rightnode.allKeys != {}
+//       && (forall key :: key in allKeys ==> Keys.lt(key, pivot))
+//       && (forall key :: key in rightnode.allKeys ==> Keys.lte(pivot, key))
+//     }
+      
+//     method Split() returns (ghost wit: Key, pivot: Key, rightnode: Node)
+//       requires WF()
+//       requires Full()
+//       ensures SplitEnsures(old(Interpretation()), pivot, rightnode)
+//       ensures allKeys <= old(allKeys)
+//       ensures rightnode.allKeys <= old(allKeys)
+//       ensures pivot in old(allKeys)
+//       ensures wit in old(allKeys)
+//       ensures Keys.lt(wit, pivot)
+//       ensures subtreeObjects <= old(subtreeObjects)
+//       ensures subtreeObjects !! rightnode.subtreeObjects
+//       ensures fresh(rightnode.subtreeObjects - old(subtreeObjects))
+//       modifies this
+//   }
+
+//   datatype NodeBox = NodeBox(node: Node?)
+
+//   class Leaf extends Node {
+//     var nkeys : uint64
+//     var keys: array<Key>
+//     var values: array<Value>
+
+//     function ToImmutableNode() : (result: ImmutableNode)
+//       ensures result.ImmutableLeaf?
+//       reads this, subtreeObjects
+//       decreases subtreeObjects, 0
+//     {
+//       ImmutableLeaf(allKeys, keys[..nkeys], values[..nkeys])
+//     }
+    
+//     predicate WF()
+//       reads this, subtreeObjects
+//       ensures WFLEaf() ==> this in subtreeObjects
+//       decreases subtreeObjects, 0
+//     {
+//       && subtreeObjects == {this, keys, values}
+//       && keys != values
+//       && keys.Length == MaxKeysPerLeaf() as int
+//       && values.Length == MaxKeysPerLeaf() as int
+//       && 0 <= nkeys <= keys.Length as uint64
+//       && WFLeaf(ToImmutableNode())
+//     }
+
+//     function Interpretation() : map<Key, Value>
+//       requires WF()
+//       reads this, subtreeObjects
+//       decreases subtreeObjects
+//     {
+//       InterpretationLeaf(ToImmutableNode())
+//     }
+
+//     method Query(needle: Key) returns (result: QueryResult)
+//       requires WF()
+//       ensures needle in Interpretation() ==> result == Found(Interpretation()[needle])
+//       ensures needle !in Interpretation() ==> result == NotFound
+//       //ensures result == QueryDef(needle)
+//       decreases subtreeObjects
+//     {
+//       //Keys.reveal_IsStrictlySorted();
+//       var posplus1: uint64 := Keys.ArrayLargestLtePlus1(keys, 0, nkeys, needle);
+//       if 1 <= posplus1 && keys[posplus1-1] == needle {
+//         result := Found(values[posplus1-1]);
+//       } else {
+//         result := NotFound;
+//       }
+//     }
+
+//     predicate method Full()
+//       requires WF()
+//       reads this, subtreeObjects
+//     {
+//       nkeys >= MaxKeysPerLeaf()
+//     }
+    
+//     method Insert(key: Key, value: Value)
+//       requires WF()
+//       requires !Full()
+//       ensures WF()
+//       ensures Interpretation() == old(Interpretation())[key := value]
+//       ensures allKeys == old(allKeys) + {key}
+//       ensures fresh(subtreeObjects-old(subtreeObjects))
+//       modifies this, subtreeObjects
+//       decreases allKeys
+//     {
+//       var posplus1 := Keys.ArrayLargestLtePlus1(keys, 0, nkeys, key);
+
+//       if 1 <= posplus1 && keys[posplus1-1] == key {
+//         values[posplus1-1] := value;
+//       } else {
+//         ghost var oldkeys := keys[..nkeys];
+//         Arrays.Insert(keys, nkeys, key, posplus1);
+//         Arrays.Insert(values, nkeys, value, posplus1);
+//         nkeys := nkeys + 1;
+//         allKeys := allKeys + {key};
+
+//         InsertMultiset(oldkeys, key, posplus1 as int); // OBSERVE
+//         Keys.strictlySortedInsert(oldkeys, key, posplus1 as int - 1); // OBSERVE
+//         Keys.PosEqLargestLte(keys[..nkeys], key, posplus1 as int);
+//         forall key' |  key' != key && key' in old(Interpretation())
+//           ensures key' in Interpretation() && Interpretation()[key'] == old(Interpretation())[key']
+//         {
+//           var i: int := Keys.LargestLte(old(keys[..nkeys]), key');
+//           //assert 0 <= i;
+//           if i < posplus1 as int {
+//             //assert keys[i] == key';
+//             Keys.PosEqLargestLte(keys[..nkeys], key', i);
+//           } else {
+//             //assert keys[i+1] == key';
+//             Keys.PosEqLargestLte(keys[..nkeys], key', i+1);
+//           }
+//         }
+//         forall key' | key' != key && key' in Interpretation()
+//           ensures key' in old(Interpretation()) && old(Interpretation())[key'] == Interpretation()[key']
+//         {
+//           var i: int := Keys.LargestLte(keys[..nkeys], key');
+//           if i < posplus1 as int {
+//             Keys.PosEqLargestLte(old(keys[..nkeys]), key', i);
+//           } else {
+//             Keys.PosEqLargestLte(old(keys[..nkeys]), key', i-1);
+//           }
+//         }
+//       }
+//     }
+
+//     method Split() returns (ghost wit: Key, pivot: Key, rightnode: Node)
+//       requires WF()
+//       requires Full()
+//       ensures SplitEnsures(old(Interpretation()), pivot, rightnode)
+//       ensures allKeys <= old(allKeys)
+//       ensures rightnode.allKeys <= old(allKeys)
+//       ensures pivot in old(allKeys)
+//       ensures wit in old(allKeys)
+//       ensures Keys.lt(wit, pivot)
+//       ensures subtreeObjects <= old(subtreeObjects)
+//       ensures subtreeObjects !! rightnode.subtreeObjects
+//       ensures fresh(rightnode.subtreeObjects - old(subtreeObjects))
+//       modifies this
+//     {
+//       var right := new Leaf();
+//       var boundary := nkeys/2;
+//       Arrays.Memcpy(right.keys, 0, keys[boundary..nkeys]); // FIXME: remove conversion to seq
+//       Arrays.Memcpy(right.values, 0, values[boundary..nkeys]); // FIXME: remove conversion to seq
+//       right.nkeys := nkeys - boundary;
+//       nkeys := boundary;
+//       allKeys := set key | key in multiset(keys[..nkeys]);
+//       right.allKeys := set key | key in multiset(right.keys[..right.nkeys]);
+//       assert keys[0] in allKeys;
+//       assert right.keys[0] in right.allKeys;
+//       wit := keys[0];
+//       pivot := right.keys[0];
+//       rightnode := right;
+
+//       assert keys[..nkeys] == old(keys[..nkeys])[..nkeys];
+//       Keys.StrictlySortedSubsequence(old(keys[..nkeys]), 0, nkeys as int);
+//       assert WF();
+//       assert right.keys[..right.nkeys] == old(keys[..nkeys])[boundary..old(nkeys)];
+//       Keys.StrictlySortedSubsequence(old(keys[..nkeys]), boundary as int, old(nkeys) as int);
+//       assert Keys.IsStrictlySorted(right.keys[..right.nkeys]);
+//       assert right.WF();
+//       Keys.IsStrictlySortedImpliesLt(old(keys[..nkeys]), 0, boundary as int);
+//       forall i | 0 <= i < nkeys
+//         ensures Keys.lt(keys[i], pivot)
+//       {
+//         Keys.IsStrictlySortedImpliesLt(old(keys[..nkeys]), i as int, boundary as int);
+//       }
+//       ghost var mergedint := MergeMaps(Interpretation(), pivot, rightnode.Interpretation());
+//       forall key | key in old(Interpretation())
+//         ensures key in mergedint && mergedint[key] == old(Interpretation())[key]
+//       {
+//         if Keys.lt(key, pivot) {
+//           assert Keys.LargestLte(old(keys[..nkeys]), key) < boundary as int;
+//         } else {
+//         }
+//       }
+//     }
+      
+//     constructor()
+//       ensures WF()
+//       ensures Interpretation() == map[]
+//       ensures !Full()
+//       ensures fresh(keys)
+//       ensures fresh(values)
+//     {
+//       nkeys := 0;
+//       keys := new Key[MaxKeysPerLeaf()](_ => DefaultKey());
+//       values := new Value[MaxKeysPerLeaf()](_ => DefaultValue());
+//       allKeys := {};
+//       subtreeObjects := {this, keys, values};
+//     }
+//   }
+
+//   class Index extends Node {
+//     var nchildren: uint64
+//     var pivots: array<Key>
+//     var children: array<NodeBox>
+
+//     predicate WF()
+//       reads this, subtreeObjects
+//       ensures WF() ==> this in subtreeObjects
+//       decreases subtreeObjects, 0
+//     {
+//       && {this, pivots, children} <= subtreeObjects
+//       && pivots.Length == (MaxChildren() as int) - 1
+//       && children.Length == MaxChildren() as int
+//       && 1 <= nchildren <= MaxChildren()
+//       && (forall i :: 0 <= i < nchildren ==> children[i].node != null)
+//       && (forall i :: 0 <= i < nchildren ==> children[i].node in subtreeObjects)
+//       && (forall i {:trigger children[i].node.subtreeObjects} :: 0 <= i < nchildren as int ==> children[i].node.subtreeObjects < subtreeObjects)
+//       && (forall i {:trigger children[i].node.subtreeObjects} :: 0 <= i < nchildren as int ==> {this, pivots, children} !! children[i].node.subtreeObjects)
+//       && (forall i, j {:trigger children[i].node.subtreeObjects, children[j].node.subtreeObjects} :: 0 <= i < j < nchildren as int ==> children[i].node.subtreeObjects !! children[j].node.subtreeObjects)
+//       && WFIndex(ToImmutableNode())
+//     }
+
+//     // lemma AllKeysStrictlyDecreasing()
+//     //   requires WF()
+//     //   ensures forall i :: 0 <= i < nchildren ==> children[i].node.allKeys < allKeys
+//     // {
+//     //   forall i | 0 <= i < nchildren
+//     //     ensures children[i].node.allKeys < allKeys
+//     //   {
+//     //     var i' := if i < nchildren-1 then i+1 else 0;
+//     //     assert i' != i;
+//     //     assert children[i].node.allKeys !! children[i'].node.allKeys;
+//     //     assert children[i].node.allKeys <= 
+//     //     assert children[i].node.allKeys <= allKeys;
+//     //   }
+//     // }
+    
+//     // function QueryDef(needle: Key) : QueryResult
+//     //   requires WF()
+//     //   reads this, subtreeObjects
+//     //   decreases subtreeObjects
+//     // {
+//     //   var pos := Keys.LargestLte(pivots[..nchildren-1], needle);
+//     //   children[pos + 1].node.QueryDef(needle)
+//     // }
+    
+//     function Interpretation() : (result: map<Key, Value>)
+//       requires WF()
+//       // ensures forall key :: QueryDef(key).Found? ==> MapsTo(result, key, QueryDef(key).value)
+//       // ensures forall key :: QueryDef(key).NotFound? ==> key !in Interpretation()
+//       reads this, subtreeObjects
+//       decreases subtreeObjects
+//     {
+//       // This is just to prove finiteness.  Thanks to James Wilcox for the trick:
+//       // https://stackoverflow.com/a/47585360
+//       var allkeys := set key, i | 0 <= i < nchildren && key in children[i].node.Interpretation() :: key;
+//       var result := map key |
+//         && key in allkeys
+//         && key in children[Keys.LargestLte(pivots[..nchildren-1], key) + 1].node.Interpretation()
+//         :: children[Keys.LargestLte(pivots[..nchildren-1], key) + 1].node.Interpretation()[key];
+
+//       // assert forall key :: QueryDef(key).Found? ==> key in children[Keys.LargestLte(pivots[..nchildren-1], key)+1].node.Interpretation();
+        
+//       result
+//     }
+
+//     method Query(needle: Key) returns (result: QueryResult)
+//       requires WF()
+//       ensures needle in Interpretation() ==> result == Found(Interpretation()[needle])
+//       ensures needle !in Interpretation() ==> result == NotFound
+//       // ensures result == QueryDef(needle)
+//       decreases subtreeObjects
+//     {
+//       var posplus1 := Keys.ArrayLargestLtePlus1(pivots, 0, nchildren-1, needle);
+//       result := children[posplus1].node.Query(needle);
+//     }
+
+//     predicate method Full()
+//       requires WF()
+//       reads this, subtreeObjects
+//     {
+//       nchildren == MaxChildren()
+//     }
+
+//     static lemma SplitChildIsCorrect()
+    
+//     method SplitChild(key: Key, childidx: uint64) returns (newchildidx: uint64)
+//       requires WF()
+//       requires !Full()
+//       requires childidx as int == 1 + Keys.LargestLte(pivots[..nchildren-1], key)
+//       requires children[childidx].node.Full()
+//       ensures WF()
+//       ensures Interpretation() == old(Interpretation())
+//       ensures newchildidx as int == 1 + Keys.LargestLte(pivots[..nchildren-1], key)
+//       ensures !children[newchildidx].node.Full()
+//       ensures allKeys == old(allKeys)
+//       ensures fresh(subtreeObjects-old(subtreeObjects))
+//       modifies this, pivots, children, children[childidx].node
+//     {
+//       ghost var oldchildren := children[..nchildren];
+      
+//       var wit, pivot, right := children[childidx].node.Split();
+//       Arrays.Insert(pivots, nchildren - 1, pivot, childidx);
+//       Arrays.Insert(children, nchildren, NodeBox(right), childidx + 1);
+//       nchildren := nchildren + 1;
+//       subtreeObjects := subtreeObjects + right.subtreeObjects;
+//       if Keys.lte(pivot, key) {
+//         newchildidx := childidx + 1;
+//       } else {
+//         newchildidx := childidx;
+//       }
+
+//       Keys.LargestLteIsUnique(old(pivots[..nchildren-1]), pivot, childidx as int - 1);
+//       Keys.strictlySortedInsert(old(pivots[..nchildren-1]), pivot, childidx as int - 1);
+
+//       assert forall i :: 0 <= i < childidx as int ==> children[i] == oldchildren[i];
+//       assert children[childidx as int + 1].node == right;
+//       assert forall i :: childidx as int + 1 < i < nchildren as int  ==> children[i] == oldchildren[i-1];
+//       forall i: int, j: int {:trigger children[i].node.subtreeObjects, children[j].node.subtreeObjects}
+//       | 0 <= i < j < nchildren as int
+//         ensures children[i].node.subtreeObjects !! children[j].node.subtreeObjects
+//       {
+//         if                                   j  < childidx as int {
+//         } else if                            j == childidx as int {
+//         } else if i  < childidx as int     && j == childidx as int + 1 {
+//         } else if i == childidx as int     && j == childidx as int + 1 {
+//         } else if i  < childidx as int     && j  > childidx as int + 1 {
+//         } else if i == childidx as int     && j  > childidx as int + 1 {
+//         } else if i == childidx as int + 1 && j  > childidx as int + 1 {
+//         } else {
+//         }
+//       }
+//       // forall i: int, key | 0 <= i < (nchildren as int)-1 && key in children[i].node.allKeys
+//       //   ensures Keys.lt(key, pivots[i])
+//       // {
+//       //   if childidx as int + 1 < i {
+//       //     assert children[i] == old(children[i-1]);
+//       //   }
+//       // }
+//       // forall i: int, key | 0 < i < nchildren as int && key in children[i].node.allKeys
+//       //   ensures Keys.lt(pivots[i-1], key)
+//       // {
+//       //   if i < childidx as int {
+//       //     assert Keys.lt(pivots[i-1], key);
+//       //   } else if i == childidx as int {
+//       //     assert Keys.lt(pivots[i-1], key);
+//       //   } else if i == childidx as int + 1 {
+//       //     assert Keys.lt(pivots[i-1], key);
+//       //   } else {
+//       //     assert Keys.lt(pivots[i-1], key);
+//       //   }
+//       // }
+//       assert WF();
+        
+//       forall key | key in old(Interpretation())
+//         ensures key in Interpretation() && Interpretation()[key] == old(Interpretation()[key])
+//       {
+//         var llte: int := Keys.LargestLte(old(pivots[..nchildren-1]), key);
+//         assert key in old(children[llte+1].node.Interpretation());
+//         assert old(children[llte+1].node.Interpretation()[key]) == old(Interpretation()[key]);
+//         if llte < childidx as int {
+//           assert key in Interpretation() && Interpretation()[key] == old(Interpretation()[key]);
+//         } else if llte == childidx as int {
+//           if Keys.lt(key, pivot) {
+//             assert key in Interpretation() && Interpretation()[key] == old(Interpretation()[key]);
+//           } else {
+//             assert key in Interpretation() && Interpretation()[key] == old(Interpretation()[key]);
+//           }
+//         } else {
+//           assert key in Interpretation() && Interpretation()[key] == old(Interpretation()[key]);
+//         }
+//       }
+//       forall key | key in Interpretation()
+//         ensures key in old(Interpretation()) && Interpretation()[key] == old(Interpretation()[key])
+//       {
+//         var llte: int := Keys.LargestLte(pivots[..nchildren-1], key);
+//         if llte < childidx as int {
+//         } else if llte == childidx as int {
+//         } else if llte == childidx as int + 1 {
+//         } else {
+//         }
+//       }
+//     }
+    
+//     method Insert(key: Key, value: Value)
+//       requires WF()
+//       requires !Full()
+//       ensures WF()
+//       ensures Interpretation() == old(Interpretation())[key := value]
+//       ensures allKeys == old(allKeys) + {key}
+//       ensures fresh(subtreeObjects - old(subtreeObjects))
+//       modifies this, subtreeObjects
+//       decreases allKeys
+//     {
+//       var posplus1 := Keys.ArrayLargestLtePlus1(pivots, 0, nchildren - 1, key);
+//       var childidx := (posplus1) as uint64;
+//       if children[posplus1].node.Full() {
+//         childidx := SplitChild(key, childidx);
+//       }
+//       //AllKeysStrictlyDecreasing();
+//       children[childidx].node.Insert(key, value);
+//       subtreeObjects := subtreeObjects + children[childidx].node.subtreeObjects;
+//       allKeys := allKeys + {key};
+//       forall key' | key' in old(Interpretation()) && key' != key
+//         ensures key' in Interpretation() && Interpretation()[key'] == old(Interpretation()[key'])
+//       {
+//         var i :| 0 <= i < old(nchildren) && key' in old(children[i].node.Interpretation());
+//       }
+      
+//     }
+
+//     function UnionSubtreeObjects() : set<object>
+//       requires nchildren as int <= children.Length
+//       requires forall i :: 0 <= i < nchildren ==> children[i].node != null
+//       reads this, children, set i | 0 <= i < nchildren :: children[i].node
+//     {
+//       set o, i | 0 <= i < nchildren && o in children[i].node.subtreeObjects :: o
+//     }
+    
+//     method Split() returns (ghost wit: Key, pivot: Key, rightnode: Node)
+//       requires WF()
+//       requires Full()
+//       ensures SplitEnsures(old(Interpretation()), pivot, rightnode)
+//       ensures allKeys <= old(allKeys)
+//       ensures rightnode.allKeys <= old(allKeys)
+//       ensures pivot in old(allKeys)
+//       ensures wit in old(allKeys)
+//       ensures Keys.lt(wit, pivot)
+//       ensures subtreeObjects <= old(subtreeObjects)
+//       ensures subtreeObjects !! rightnode.subtreeObjects
+//       ensures fresh(rightnode.subtreeObjects - old(subtreeObjects))
+//       modifies this
+//     {
+//       var right := new Index();
+//       var boundary := nchildren/2;
+//       Arrays.Memcpy(right.pivots, 0, pivots[boundary..nchildren-1]); // FIXME: remove conversion to seq
+//       Arrays.Memcpy(right.children, 0, children[boundary..nchildren]); // FIXME: remove conversion to seq
+//       right.nchildren := nchildren - boundary;
+//       nchildren := boundary;
+//       subtreeObjects := {this, pivots, children} + UnionSubtreeObjects();
+//       right.subtreeObjects := right.subtreeObjects + right.UnionSubtreeObjects();
+
+//       pivot := pivots[boundary-1];
+
+//       right.allKeys := set k | k in allKeys && Keys.lte(pivot, k);
+//       allKeys := set k | k in allKeys && Keys.lt(k, pivot);
+      
+//       wit := right.pivots[0];
+//       rightnode := right;
+//       AssumeFalse();
+      
+//       // Keys.reveal_IsStrictlySorted();
+//       // assert WF();
+//       // assert rightnode.WF();
+//       // assert MergeMaps(Interpretation(), pivot, rightnode.Interpretation()) == old(Interpretation());
+//     }
+
+//     constructor()
+//       ensures nchildren == 0
+//       ensures pivots.Length == (MaxChildren() as int)-1
+//       ensures children.Length == (MaxChildren() as int)
+//       ensures forall i :: 0 <= i < children.Length ==> children[i].node == null
+//       ensures subtreeObjects == {this, pivots, children}
+//       ensures allKeys == {}
+//       ensures fresh(pivots)
+//       ensures fresh(children)
+//     {
+//       pivots := new Key[MaxChildren()-1](_ => DefaultKey());
+//       children := new NodeBox[MaxChildren()](_ => NodeBox(null));
+//       nchildren := 0;
+//       subtreeObjects := {this, pivots, children};
+//       allKeys := {};
+//     }
+//   }
+
+//   class MutableBtree {
+//     var root: Node
+
+//     function Interpretation() : map<Key, Value>
+//       requires root.WF()
+//       reads this, root, root.subtreeObjects
+//     {
+//       root.Interpretation()
+//     }
+
+//     method Query(needle: Key) returns (result: QueryResult)
+//       requires root.WF()
+//       ensures result == NotFound ==> needle !in Interpretation()
+//       ensures result.Found? ==> needle in Interpretation() && Interpretation()[needle] == result.value
+//     {
+//       result := root.Query(needle);
+//     }
+
+//     method Insert(key: Key, value: Value)
+//       requires root.WF()
+//       ensures root.WF()
+//       ensures Interpretation() == old(Interpretation())[key := value]
+//       modifies this, root, root.subtreeObjects
+//     {
+//       if root.Full() {
+//         var newroot := new Index();
+//         newroot.children[0] := NodeBox(root);
+//         newroot.nchildren := 1;
+//         newroot.subtreeObjects := newroot.subtreeObjects + root.subtreeObjects;
+//         newroot.allKeys := root.allKeys;
+//         root := newroot;
+//       }
+//       AssumeFalse();
+//       root.Insert(key, value);
+//     }
+    
+//     constructor()
+//       ensures root.WF()
+//       ensures Interpretation() == map[]
+//     {
+//       root := new Leaf();
+//     }
+//   }
+// }
+
+// module TestMutableBtree refines MutableBtree {
+//   import Keys = Uint64_Order
+//   type Value = uint64
+
+//   function method MaxKeysPerLeaf() : uint64 { 64 }
+//   function method MaxChildren() : uint64 { 64 }
+
+//   function method DefaultValue() : Value { 0 }
+//   function method DefaultKey() : Key { 0 }
+// }
+
+// module MainModule {
+//   import opened NativeTypes
+//   import TestMutableBtree
+    
+//   method Main()
+//   {
+//     // var n: uint64 := 1_000_000;
+//     // var p: uint64 := 300_007;
+//     var n: uint64 := 10_000_000;
+//     var p: uint64 := 3_000_017;
+//     // var n: uint64 := 100_000_000;
+//     // var p: uint64 := 1_073_741_827;
+//     var t := new TestMutableBtree.MutableBtree();
+//     var i: uint64 := 0;
+//     while i < n
+//       invariant 0 <= i <= n
+//       invariant t.root.WF()
+//       modifies t, t.root, t.root.subtreeObjects
+//     {
+//       t.Insert((i * p) % n , i);
+//       i := i + 1;
+//     }
+
+//     // i := 0;
+//     // while i < n
+//     //   invariant 0 <= i <= n
+//     // {
+//     //   var needle := (i * p) % n;
+//     //   var qr := t.Query(needle);
+//     //   if qr != TestMutableBtree.Found(i) {
+//     //     print "Test failed";
+//   //   } else {
+//   //     //print "Query ", i, " for ", needle, "resulted in ", qr.value, "\n";
+//   //   }
+//   //   i := i + 1;
+//   // }
+
+//   // i := 0;
+//   // while i < n
+//   //   invariant 0 <= i <= n
+//   // {
+//   //   var qr := t.Query(n + ((i * p) % n));
+//   //   if qr != TestMutableBtree.NotFound {
+//   //     print "Test failed";
+//   //   } else {
+//   //     //print "Didn't return bullsh*t\n";
+//   //   }
+//   //   i := i + 1;
+//   // }
+//     print "PASSED\n";
+//   }
 } 
